

CH 6. 선형 미분 방정식

6.1 제 1계 선형 미분 방정식 (First-order linear coupled differential Equation)

General form

$$x_1'(t) = a_{11}(t)x_1(t) + a_{12}(t)x_2(t) + \dots + a_{1n}(t)x_n(t) + g_1(t)$$

$$x_2'(t) = a_{21}(t)x_1(t) + a_{22}(t)x_2(t) + \dots + a_{2n}(t)x_n(t) + g_2(t)$$

\vdots

$$x_m'(t) = a_{m1}(t)x_1(t) + a_{m2}(t)x_2(t) + \dots + a_{mn}(t)x_n(t) + g_m(t)$$

Let

$$X(t) = \begin{pmatrix} x_1(t) \\ x_2(t) \\ \vdots \\ x_n(t) \end{pmatrix}$$

$$A(t) = \begin{pmatrix} a_{11}(t) & a_{12}(t) & \dots & a_{1n}(t) \\ a_{21}(t) & a_{22}(t) & \dots & a_{2n}(t) \\ \vdots & \vdots & \ddots & \vdots \\ a_{m1}(t) & a_{m2}(t) & \dots & a_{mn}(t) \end{pmatrix}$$

$$G(t) = \begin{pmatrix} g_1(t) \\ g_2(t) \\ \vdots \\ g_m(t) \end{pmatrix}$$

\Rightarrow General Form

$$\underline{X'(t) = A(t)X(t) + G(t)}$$

If $G(t) = 0$, Homogeneous differential Equation

If $G(t) \neq 0$, non-homogeneous differential Equation

p227

(9.1.1)

$$x_1' = 3x_1 + 3x_2 + 8$$

$$x_2' = x_1 + 5x_2 + 4e^{3t}$$

$$\Rightarrow \begin{pmatrix} x_1 \\ x_2 \end{pmatrix}' = \begin{pmatrix} 3 & 3 \\ 1 & 5 \end{pmatrix} \begin{pmatrix} x_1 \\ x_2 \end{pmatrix} + \begin{pmatrix} 8 \\ 4e^{3t} \end{pmatrix}$$

Solution

$$x_1(t) = 3e^{2t} + e^{6t} - 4e^{3t} - \frac{10}{2}$$

 \Rightarrow 행렬식!!

$$x_2(t) = -e^{2t} + e^{6t} + \frac{7}{2}$$

$$X(t) = \begin{pmatrix} x_1(t) \\ x_2(t) \end{pmatrix} = \begin{pmatrix} 3e^{2t} + e^{6t} - 4e^{3t} - \frac{10}{2} \\ -e^{2t} + e^{6t} + \frac{7}{2} \end{pmatrix}$$

solution vector

*

p228

9.1.1

If $a_{ij}(t)$ and $g_j(t)$ are continuous, the differential equation

$$X' = AX + G \quad X(t_0) = X_0$$

has unique solution.

Ex 6.2 : Homogeneous equation

If X_1, X_2, \dots, X_k are solution of the homogeneous equation

$$X' = A X,$$

$C_1 X_1 + C_2 X_2 + \dots + C_k X_k$ is also solution.

p228

(Ex 6.3)

$$X' = \begin{pmatrix} 1 & -4 \\ 1 & 5 \end{pmatrix} X$$

$$X_1 = \begin{pmatrix} -2e^{2t} \\ e^{2t} \end{pmatrix}$$

$$X_2 = \begin{pmatrix} (1-2t)e^{2t} \\ te^{2t} \end{pmatrix}$$

⇒ 행의식할것!!

solution vector

Then

$$C_1 X_1 + C_2 X_2 = \begin{pmatrix} -[2C_1 t + (2C_2 - C_1)]e^{2t} \\ (C_2 t + C_1)e^{2t} \end{pmatrix}$$

⇒ 행의식할것!!

is also solution vector.

p230

24.6.4: General solution of homogeneous equation

Consider a homogeneous equation

$$X' = A X,$$

where A is $n \times n$ matrix.

Let $X_1(t), X_2(t), \dots, X_m(t)$ are solution vectors of the

homogeneous equation and linearly-independent.

Then the general solution of the homogeneous equation is

$$X = C_1 X_1(t) + C_2 X_2(t) + \dots + C_m X_m(t)$$

* Linearly-independent condition:

$$\text{Let } X_1(t) = \begin{pmatrix} x_{11}(t) \\ x_{12}(t) \\ \vdots \\ x_{1n}(t) \end{pmatrix} \quad X_2(t) = \begin{pmatrix} x_{21}(t) \\ x_{22}(t) \\ \vdots \\ x_{2n}(t) \end{pmatrix} \quad \dots \quad X_m(t) = \begin{pmatrix} x_{m1}(t) \\ x_{m2}(t) \\ \vdots \\ x_{mn}(t) \end{pmatrix}$$

Consider $n \times m$ determinant

$$W = \begin{vmatrix} x_{11}(t) & x_{21}(t) & \dots & x_{m1}(t) \\ x_{12}(t) & x_{22}(t) & \dots & x_{m2}(t) \\ \vdots & \vdots & \dots & \vdots \\ x_{1n}(t) & x_{2n}(t) & \dots & x_{mn}(t) \end{vmatrix}$$

If $W \neq 0$, $\{X_1, X_2, \dots, X_m\}$ is linearly-independent

If $W = 0$, $\{X_1, X_2, \dots, X_m\}$ is linearly-dependent.

#

p230 (01/2016.4)

$$X' = \begin{pmatrix} 1 & -4 \\ 1 & 5 \end{pmatrix} X$$

$$X_1 = \begin{pmatrix} -2e^{3t} \\ e^{3t} \end{pmatrix}$$

$$X_2 = \begin{pmatrix} (1-2t)e^{2t} \\ te^{2t} \end{pmatrix}$$

solution vectors

$$W = \begin{vmatrix} -2e^{3t} & (1-2t)e^{2t} \\ e^{3t} & te^{2t} \end{vmatrix} = -e^{6t} \neq 0$$

Therefore $\{X_1, X_2\}$ is linearly independent.

General solution

$$X(t) = C_1 X_1 + C_2 X_2$$

$$\Rightarrow X(t) = C_1 \begin{pmatrix} -2e^{3t} \\ e^{3t} \end{pmatrix} + C_2 \begin{pmatrix} (1-2t)e^{2t} \\ te^{2t} \end{pmatrix}$$

$$= \begin{pmatrix} -2C_1 e^{3t} + C_2 (1-2t)e^{2t} \\ C_1 e^{3t} + C_2 t e^{2t} \end{pmatrix}$$

$$= \begin{pmatrix} -2e^{3t} & (1-2t)e^{2t} \\ e^{3t} & te^{2t} \end{pmatrix} \begin{pmatrix} C_1 \\ C_2 \end{pmatrix}$$

$$= Q(t) \begin{pmatrix} C_1 \\ C_2 \end{pmatrix}$$

$$\Omega(t) = \begin{pmatrix} -2e^{3t} & (1-2t)e^{3t} \\ e^{3t} & te^{3t} \end{pmatrix}$$

: 기본행렬 (fundamental matrix)

*

p231

(0912116.5)

$$X' = \begin{pmatrix} 1 & -4 \\ 1 & 5 \end{pmatrix} X \quad X(0) = \begin{pmatrix} -2 \\ 2 \end{pmatrix}$$

general solution

$$X(t) = \Omega(t) \begin{pmatrix} c_1 \\ c_2 \end{pmatrix}$$

$$= \begin{pmatrix} -2e^{3t} & (1-2t)e^{3t} \\ e^{3t} & te^{3t} \end{pmatrix} \begin{pmatrix} c_1 \\ c_2 \end{pmatrix}$$

$$X(0) = \begin{pmatrix} -2 & 1 \\ 1 & 0 \end{pmatrix} \begin{pmatrix} c_1 \\ c_2 \end{pmatrix} = \begin{pmatrix} -2 \\ 2 \end{pmatrix}$$

$$-2c_1 + c_2 = -2$$

$$c_1 = 3$$

$$\Rightarrow c_1 = 3$$

$$c_2 = 4$$

$$\Rightarrow X(t) = \Omega(t) \begin{pmatrix} 3 \\ 4 \end{pmatrix} = \begin{pmatrix} -2e^{3t} & (1-2t)e^{3t} \\ e^{3t} & te^{3t} \end{pmatrix} \begin{pmatrix} 3 \\ 4 \end{pmatrix}$$

$$= \begin{pmatrix} -6e^{3t} + 4(1-2t)e^{3t} \\ 3e^{3t} + 4te^{3t} \end{pmatrix} \quad *$$

16.21.6.5 : non-homogeneous Equation

Let us consider non-homogeneous differential Equation:

$$X' = AX + G$$

Let $X = \Omega C$ be a general solution of the homogeneous equation $X' = AX$, and Φ_p be a particular solution of the non-homogeneous equation $X' = AX + G$. Then the general solution of $X' = AX + G$ is

$$X = \Omega C + \Phi_p$$

* 상수계수 Homogeneous coupled linear differential Equation

$$X' = A X \quad \text{--- ①}$$

A : constant $n \times n$ matrix

Let

$$X = \xi e^{\lambda t} \quad \text{--- ②}$$

ξ : $(n \times 1)$ constant matrix

② \rightarrow ①

$$\lambda \xi e^{\lambda t} = A \xi e^{\lambda t}$$

$$\Rightarrow A \xi = \lambda \xi \quad \text{--- ③}$$

λ : eigenvalue of A

ξ : eigenvector of A

7.4.6.6

$$X' = A X \quad \text{의 일반해}$$

$$A \text{의 eigenvalue} = \{\lambda_1, \lambda_2, \dots, \lambda_n\}$$

$$A \text{의 eigenvector} = \{\xi_1, \xi_2, \dots, \xi_n\}$$

$$X = c_1 \xi_1 e^{\lambda_1 t} + c_2 \xi_2 e^{\lambda_2 t} + \dots + c_n \xi_n e^{\lambda_n t}$$

p232

(5/12/16.6)

$$X' = \begin{pmatrix} 4 & 2 \\ 3 & 3 \end{pmatrix} X$$

$$A = \begin{pmatrix} 4 & 2 \\ 3 & 3 \end{pmatrix}$$

* eigenvalue

$$\begin{vmatrix} 4-\lambda & 2 \\ 3 & 3-\lambda \end{vmatrix} = 0$$

$$\lambda = 1 \text{ and } 6$$

* eigenvector

$$(i) \lambda = 1$$

$$\begin{pmatrix} 4 & 2 \\ 3 & 3 \end{pmatrix} \begin{pmatrix} a \\ b \end{pmatrix} = \begin{pmatrix} a \\ b \end{pmatrix}$$

$$3a + 2b = 0$$

$$a = 2, \quad b = -3 \quad \Rightarrow \quad \underline{z}_1 = \begin{pmatrix} 2 \\ -3 \end{pmatrix}$$

$$(ii) \lambda = 6$$

$$\begin{pmatrix} 4 & 2 \\ 3 & 3 \end{pmatrix} \begin{pmatrix} a \\ b \end{pmatrix} = 6 \begin{pmatrix} a \\ b \end{pmatrix}$$

$$a = b$$

$$\Rightarrow a = b = 1 \quad \Rightarrow \quad \underline{z}_2 = \begin{pmatrix} 1 \\ 1 \end{pmatrix}$$

$$X(t) = c_1 \underline{z}_1 e^{\lambda_1 t} + c_2 \underline{z}_2 e^{\lambda_2 t}$$

$$= c_1 \begin{pmatrix} 2 \\ -3 \end{pmatrix} e^t + c_2 \begin{pmatrix} 1 \\ 1 \end{pmatrix} e^{6t}$$

$$= \begin{pmatrix} 2c_1 e^t + c_2 e^{6t} \\ -3c_1 e^t + c_2 e^{6t} \end{pmatrix} = Q(t) \begin{pmatrix} c_1 \\ c_2 \end{pmatrix}$$

where

$$Q(t) = \begin{pmatrix} 2e^t & e^{6t} \\ -3e^t & e^{6t} \end{pmatrix} \quad *$$

fundamental matrix

prob (9/21/6.7)

$$x' = A x$$

$$A = \begin{pmatrix} 2 & 0 & 1 \\ 0 & -2 & -2 \\ 0 & 2 & 0 \end{pmatrix}$$

* eigenvalues

$$\begin{vmatrix} 2-\lambda & 0 & 1 \\ 0 & -2-\lambda & -2 \\ 0 & 2 & -\lambda \end{vmatrix} = 0$$

$$\lambda = 2, -1 \pm \sqrt{3}i$$

(i) $\lambda_1 = 2$

$$\begin{pmatrix} 2 & 0 & 1 \\ 0 & -2 & -2 \\ 0 & 2 & 0 \end{pmatrix} \begin{pmatrix} a \\ b \\ c \end{pmatrix} = \begin{pmatrix} a \\ b \\ c \end{pmatrix}$$

$$2a + c = 2a$$

$$-2b - 2c = 2b$$

$$\Rightarrow \vec{x}_1 = \begin{pmatrix} 1 \\ 0 \\ 0 \end{pmatrix}$$

(ii) $\lambda_2 = -1 + \sqrt{3}i$

$$\begin{pmatrix} 2 & 0 & 1 \\ 0 & -2 & -2 \\ 0 & 2 & 0 \end{pmatrix} \begin{pmatrix} a \\ b \\ c \end{pmatrix} = (-1 + \sqrt{3}i) \begin{pmatrix} a \\ b \\ c \end{pmatrix}$$

$$(-3 + \sqrt{3}i)a = c$$

$$(1 + \sqrt{3}i)b = -2c$$

$$\Rightarrow \vec{x}_2 = \begin{pmatrix} 1 \\ -2\sqrt{3}i \\ -3 + \sqrt{3}i \end{pmatrix}$$

$$(iii) \lambda_3 = -1 - \sqrt{3}i$$

$$\begin{pmatrix} 2 & 0 & 1 \\ 0 & -2 & -2 \\ 0 & 2 & 0 \end{pmatrix} \begin{pmatrix} a \\ b \\ c \end{pmatrix} = (-1 - \sqrt{3}i) \begin{pmatrix} a \\ b \\ c \end{pmatrix}$$

$$-(2 + \sqrt{3}i)a = c$$

$$2b = (-1 - \sqrt{3}i)c$$

$$\Rightarrow \xi_3 = \begin{pmatrix} 1 \\ 2\sqrt{3}i \\ -3 - \sqrt{3}i \end{pmatrix}$$

$$X = C_1 \xi_1 e^{\lambda_1 t} + C_2 \xi_2 e^{\lambda_2 t} + C_3 \xi_3 e^{\lambda_3 t}$$

$$= Q(t) \begin{pmatrix} C_1 \\ C_2 \\ C_3 \end{pmatrix}$$

where

$$Q(t) = \begin{pmatrix} e^{2t} & e^{(-1+\sqrt{3}i)t} & e^{-(1+\sqrt{3}i)t} \\ 0 & -2\sqrt{3}i e^{(-1+\sqrt{3}i)t} & 2\sqrt{3}i e^{-(1+\sqrt{3}i)t} \\ 0 & (-3+\sqrt{3}i) e^{(-1+\sqrt{3}i)t} & -(3+\sqrt{3}i) e^{-(1+\sqrt{3}i)t} \end{pmatrix}$$

Fundamental matrix

⇒ different expression

$$\begin{aligned}
 & \vec{z}_2 e^{\lambda_2 t} \\
 &= \begin{pmatrix} 1 \\ -2\sqrt{3}i \\ -3+\sqrt{3}i \end{pmatrix} e^{(-1+\sqrt{3}i)t} \\
 &= \left[\begin{pmatrix} 1 \\ 0 \\ -3 \end{pmatrix} + i \begin{pmatrix} 0 \\ -2\sqrt{3} \\ \sqrt{3} \end{pmatrix} \right] e^{-t} (\cos\sqrt{3}t + i \sin\sqrt{3}t) \\
 &= e^{-t} \left[\begin{pmatrix} 1 \\ 0 \\ -3 \end{pmatrix} \cos\sqrt{3}t - \begin{pmatrix} 0 \\ -2\sqrt{3} \\ \sqrt{3} \end{pmatrix} \sin\sqrt{3}t \right] \\
 &\quad + i e^{-t} \left[\begin{pmatrix} 1 \\ 0 \\ -3 \end{pmatrix} \sin\sqrt{3}t + \begin{pmatrix} 0 \\ -2\sqrt{3} \\ \sqrt{3} \end{pmatrix} \cos\sqrt{3}t \right]
 \end{aligned}$$

By same way

$$\begin{aligned}
 & \vec{z}_3 e^{\lambda_3 t} \\
 &= e^{-t} \left[\begin{pmatrix} 1 \\ 0 \\ -3 \end{pmatrix} \cos\sqrt{3}t - \begin{pmatrix} 0 \\ -2\sqrt{3} \\ \sqrt{3} \end{pmatrix} \sin\sqrt{3}t \right] \\
 &\quad - i e^{-t} \left[\begin{pmatrix} 1 \\ 0 \\ -3 \end{pmatrix} \sin\sqrt{3}t + \begin{pmatrix} 0 \\ -2\sqrt{3} \\ \sqrt{3} \end{pmatrix} \cos\sqrt{3}t \right]
 \end{aligned}$$

Thus we can choose to linearly-independent solutions as

$$X_1 = \vec{z}_1 e^{\lambda_1 t} = \begin{pmatrix} 1 \\ 0 \\ 0 \end{pmatrix} e^{-t}$$

$$X_2 = \frac{1}{2} [\vec{z}_2 e^{\lambda_2 t} + \vec{z}_3 e^{\lambda_3 t}] = e^{-t} \begin{pmatrix} \cos\sqrt{3}t \\ 2\sqrt{3} \sin\sqrt{3}t \\ -3 \cos\sqrt{3}t - \sqrt{3} \sin\sqrt{3}t \end{pmatrix}$$

$$X_3 = \frac{1}{2i} [\vec{z}_2 e^{\lambda_2 t} - \vec{z}_3 e^{\lambda_3 t}] = e^{-t} \begin{pmatrix} \sin\sqrt{3}t \\ -2\sqrt{3} \cos\sqrt{3}t \\ -3 \sin\sqrt{3}t + \sqrt{3} \cos\sqrt{3}t \end{pmatrix}$$

general solution

$$X = C_1 X_1 + C_2 X_2 + C_3 X_3$$

$$= Q(t) \begin{pmatrix} C_1 \\ C_2 \\ C_3 \end{pmatrix}$$

where

$$Q(t) = \begin{pmatrix} e^{2t} & e^{-t} \cos \sqrt{3}t & e^{-t} \sin \sqrt{3}t \\ 0 & 2\sqrt{3} e^{-t} \sin \sqrt{3}t & -2\sqrt{3} e^{-t} \cos \sqrt{3}t \\ 0 & -e^{-t} (2 \cos \sqrt{3}t + \sqrt{3} \sin \sqrt{3}t) & e^{-t} (-3 \sin \sqrt{3}t + \sqrt{3} \cos \sqrt{3}t) \end{pmatrix} *$$

p237

(09/31/6.8)

$$X' = \begin{pmatrix} 5 & -4 & 4 \\ 12 & -11 & 12 \\ 4 & -4 & 5 \end{pmatrix} X$$

(i) eigenvalue

$$\begin{vmatrix} 5-\lambda & -4 & 4 \\ 12 & -11-\lambda & 12 \\ 4 & -4 & 5-\lambda \end{vmatrix} = 0$$

$$\Rightarrow (\lambda+3)(\lambda-1)^2 = 0$$

$$\lambda = -3, 1 \quad (\text{2x2})$$

(i) $\lambda_1 = -3$

$$\begin{pmatrix} 5 & -4 & 4 \\ 12 & -11 & 12 \\ 4 & -4 & 5 \end{pmatrix} \begin{pmatrix} a \\ b \\ c \end{pmatrix} = -3 \begin{pmatrix} a \\ b \\ c \end{pmatrix}$$

$$\Rightarrow 2a - b + c = 0$$

$$3a - 2b + 2c = 0$$

$$\Rightarrow \vec{x}_1 = \begin{pmatrix} 1 \\ 3 \\ 1 \end{pmatrix}$$

$$(ii) \lambda_2 = 1$$

$$\begin{pmatrix} 5 & -4 & 4 \\ 12 & -11 & 10 \\ 4 & -4 & 5 \end{pmatrix} \begin{pmatrix} a \\ b \\ c \end{pmatrix} = \begin{pmatrix} a \\ b \\ c \end{pmatrix}$$

$$a - b + c = 0$$

$$\vec{z}_1 = \begin{pmatrix} 1 \\ 1 \\ 0 \end{pmatrix} \quad \vec{z}_2 = \begin{pmatrix} 1 \\ 0 \\ -1 \end{pmatrix}$$

General solution

$$X = c_1 \vec{z}_1 e^{\lambda_1 t} + c_2 \vec{z}_2 e^{\lambda_2 t} + c_3 \vec{z}_3 e^{\lambda_3 t}$$

$$= c_1 \begin{pmatrix} 1 \\ 3 \\ 1 \end{pmatrix} e^{-3t} + c_2 \begin{pmatrix} 1 \\ 1 \\ 0 \end{pmatrix} e^t + c_3 \begin{pmatrix} 1 \\ 0 \\ -1 \end{pmatrix} e^t$$

$$= \begin{pmatrix} e^{-3t} & e^t & e^t \\ 3e^{-3t} & e^t & 0 \\ e^{-3t} & 0 & e^{-t} \end{pmatrix} \begin{pmatrix} c_1 \\ c_2 \\ c_3 \end{pmatrix} \quad \#$$

(Pr 21.6.9)

$$X' = AX \quad A = \begin{pmatrix} 1 & 3 \\ -3 & 7 \end{pmatrix}$$

* eigenvalue

$$\begin{vmatrix} 1-\lambda & 3 \\ -3 & 7-\lambda \end{vmatrix} = 0$$

$$\lambda = 4 \quad (2, 2)$$

* eigenvector

$$\begin{pmatrix} 1 & 3 \\ -3 & 7 \end{pmatrix} \begin{pmatrix} a \\ b \end{pmatrix} = 4 \begin{pmatrix} a \\ b \end{pmatrix}$$

$$\Rightarrow a = b$$

$$\vec{z}_1 = \begin{pmatrix} 1 \\ 1 \end{pmatrix}$$

$$\Rightarrow X_1 = \vec{z}_1 e^{\lambda t} = \begin{pmatrix} 1 \\ 1 \end{pmatrix} e^{4t} \quad - (1)$$

How to obtain X_2 ?

Put

$$X_2 = \vec{z}_1 t e^{\lambda t} + \eta e^{\lambda t} \quad - (2)$$

Then

$$X_2' = \vec{z}_1 e^{\lambda t} + \lambda \vec{z}_1 t e^{\lambda t} + \lambda \eta e^{\lambda t} \quad - (3)$$

$$AX_2 = \underline{A \vec{z}_1 t e^{\lambda t}} + A \eta e^{\lambda t}$$

$$= \lambda \vec{z}_1$$

$$= \lambda \vec{z}_1 t e^{\lambda t} + A \eta e^{\lambda t} \quad - (4)$$

If X_0 is solution vector, $X_0' = A X_0$.

$$\Rightarrow \xi_1 e^{\lambda t} + \lambda \eta e^{\lambda t} = A \eta e^{\lambda t}$$

$$\Rightarrow (A - \lambda I) \eta = \xi_1 \quad - \textcircled{8}$$

For our case

$$\begin{pmatrix} -3 & 3 \\ -3 & 3 \end{pmatrix} \eta = \begin{pmatrix} 1 \\ 1 \end{pmatrix},$$

which gives

$$\eta = \begin{pmatrix} 1 \\ \frac{1}{2} \end{pmatrix} \quad - \textcircled{9}$$

$\textcircled{8} \rightarrow \textcircled{9}$

$$X_0 = \begin{pmatrix} 1 \\ 1 \end{pmatrix} t e^{4t} + \begin{pmatrix} 1 \\ \frac{1}{2} \end{pmatrix} e^{4t}$$

$$= \begin{pmatrix} t+1 \\ t+\frac{1}{2} \end{pmatrix} e^{4t} \quad - \textcircled{10}$$

General solution

$$X = C_1 X_1 + C_2 X_0$$

$$= \begin{pmatrix} e^{4t} & (t+1)e^{4t} \\ e^{4t} & (t+\frac{1}{2})e^{4t} \end{pmatrix} \begin{pmatrix} C_1 \\ C_2 \end{pmatrix} \quad \times$$

(11.31.6.10)

$$X' = AX \quad A = \begin{pmatrix} -2 & -1 & -5 \\ 25 & -7 & 0 \\ 0 & 1 & 3 \end{pmatrix}$$

* eigenvalue

$$\begin{vmatrix} -2-\lambda & -1 & -5 \\ 25 & -7-\lambda & 0 \\ 0 & 1 & 3-\lambda \end{vmatrix} = 0$$

$$\Rightarrow (\lambda+2)^3 = 0$$

$$\lambda = -2 \quad - \textcircled{1}$$

* eigenvector

$$\begin{pmatrix} -2 & -1 & -5 \\ 25 & -7 & 0 \\ 0 & 1 & 3 \end{pmatrix} \begin{pmatrix} a \\ b \\ c \end{pmatrix} = -2 \begin{pmatrix} a \\ b \\ c \end{pmatrix}$$

$$\Rightarrow 5a - b = 0$$

$$b + 5c = 0$$

$$\Rightarrow \vec{z}_1 = \begin{pmatrix} -1 \\ -5 \\ 1 \end{pmatrix} \quad - \textcircled{2}$$

$$\Rightarrow X_1 = \vec{z}_1 e^{\lambda t} = \begin{pmatrix} -1 \\ -5 \\ 1 \end{pmatrix} e^{-2t} \quad - \textcircled{3}$$

How to obtain X_2 and X_3 ?

Put

$$X_2 = \xi_1 t e^{\lambda t} + \eta_1 e^{\lambda t} \quad - \textcircled{5}$$

Then

$$(A - \lambda I)\eta_1 = \xi_1 \quad - \textcircled{6}$$

$$\Rightarrow \begin{pmatrix} 0 & -1 & -5 \\ 25 & -5 & 0 \\ 0 & 1 & 5 \end{pmatrix} \eta_1 = \begin{pmatrix} -1 \\ -5 \\ 1 \end{pmatrix}$$

$$\Rightarrow \eta_1 = \begin{pmatrix} -1 \\ -4 \\ 1 \end{pmatrix} \quad - \textcircled{7}$$

Thus

$$X_2 = \begin{pmatrix} -1 \\ -5 \\ 1 \end{pmatrix} t e^{-\lambda t} + \begin{pmatrix} -1 \\ -4 \\ 1 \end{pmatrix} e^{-\lambda t}$$

$$= \begin{pmatrix} -t-1 \\ -5t-4 \\ t+1 \end{pmatrix} e^{-\lambda t} \quad - \textcircled{8}$$

How to compute X_3 ? Put

$$X_3 = \frac{1}{2} \xi_1 t^2 e^{\lambda t} + \eta_2 t e^{\lambda t} + \eta_3 e^{\lambda t} \quad - (8)$$

$$X'_3 = \frac{\lambda}{2} \xi_1 t^2 e^{\lambda t} + \xi_1 t e^{\lambda t} + \eta_2 e^{\lambda t} + \lambda \eta_2 t e^{\lambda t} + \lambda \eta_3 e^{\lambda t} \quad - (9)$$

$$\begin{aligned} AX_3 &= \frac{1}{2} \underline{A \xi_1} t^2 e^{\lambda t} + A \eta_2 t e^{\lambda t} + A \eta_3 e^{\lambda t} \\ &\quad \lambda \xi_1 \\ &= \frac{\lambda}{2} \xi_1 t^2 e^{\lambda t} + A \eta_2 t e^{\lambda t} + A \eta_3 e^{\lambda t} \quad - (10) \end{aligned}$$

Since $X'_3 = AX_3$, we have

$$(A - \lambda I) \eta_2 = \xi_1 \quad - (11)$$

$$(A - \lambda I) \eta_3 = \eta_2 \quad - (12)$$

Comparing Eq. (11) with Eq. (10), we have

$$\eta_2 = \eta_1 = \begin{pmatrix} -1 \\ -4 \\ 1 \end{pmatrix} \quad - (13)$$

(12) \rightarrow (13)

$$\begin{pmatrix} 0 & -1 & -5 \\ 25 & -5 & 0 \\ 0 & 1 & 5 \end{pmatrix} \eta_3 = \begin{pmatrix} -1 \\ -4 \\ 1 \end{pmatrix}$$

$$\Rightarrow \eta_3 = \begin{pmatrix} -\frac{24}{5} \\ -4 \\ 1 \end{pmatrix} \quad - (14)$$

(13), (14) \rightarrow (8)

$$X_3 = \begin{pmatrix} -\frac{1}{2}t^2 - t - \frac{24}{5} \\ -\frac{1}{2}t^2 - 4t - 4 \\ \frac{1}{2}t^2 + t + 1 \end{pmatrix} e^{-2t} \quad - (15)$$

General solution

$$X = C_1 X_1 + C_2 X_2 + C_3 X_3$$

$$= \begin{pmatrix} -e^{-2t} & -(t+1)e^{-2t} & -(\frac{1}{2}t^2 + t + \frac{2}{5})e^{-2t} \\ -te^{-2t} & -(5t+4)e^{-2t} & -(\frac{1}{2}t^2 + 4t + 4)e^{-2t} \\ e^{-2t} & (t+1)e^{-2t} & (\frac{1}{2}t^2 + t + 1)e^{-2t} \end{pmatrix} \begin{pmatrix} C_1 \\ C_2 \\ C_3 \end{pmatrix} \quad \times$$

* eigenvalue = λ (kth $\frac{2\pi}{n}$)

$$\text{eigenvector} = \bar{z}_1$$

$$X_1(t) = \bar{z}_1 e^{\lambda t}$$

$$X_2(t) = \bar{z}_1 t e^{\lambda t} + \eta_1 e^{\lambda t}$$

$$X_3(t) = \frac{1}{2} \bar{z}_1 t^2 e^{\lambda t} + \eta_2 t e^{\lambda t} + \eta_3 e^{\lambda t}$$

$$X_4(t) = \frac{1}{3!} \bar{z}_1 t^3 e^{\lambda t} + \frac{1}{2!} \eta_4 t^2 e^{\lambda t} + \eta_5 t e^{\lambda t} + \eta_6 e^{\lambda t}$$

$$\vdots$$

$$X_k(t) = \frac{1}{(k-1)!} \bar{z}_1 t^{k-1} e^{\lambda t} + \frac{1}{(k-2)!} \eta_1 t^{k-2} e^{\lambda t} + \dots + \eta_{k-1} e^{\lambda t}$$

$$X' = A X \quad - (1)$$

If

$$A = P D P^{-1} \quad - (2)$$

where

$$D = \begin{pmatrix} \lambda_1 & 0 & 0 & \dots & 0 \\ 0 & \lambda_2 & 0 & \dots & 0 \\ \vdots & \vdots & \vdots & & \vdots \\ 0 & 0 & 0 & \dots & \lambda_m \end{pmatrix}, \quad - (3)$$

Eg. (1) becomes

$$X' = P D P^{-1} X \quad (4)$$

Put

$$Z = P^{-1} X \quad (5)$$

(5) \rightarrow (4)

$$Z' = D Z \quad (6)$$

Thus

$$Z = Q_D(t) \begin{pmatrix} c_1 \\ c_2 \\ \vdots \\ c_m \end{pmatrix} \quad (7)$$

where

$$Q_D(t) = \begin{pmatrix} e^{\lambda_1 t} & 0 & \dots & 0 \\ 0 & e^{\lambda_2 t} & \dots & 0 \\ \vdots & \vdots & & \vdots \\ 0 & 0 & \dots & e^{\lambda_m t} \end{pmatrix} \quad - (8)$$

(7) \rightarrow (5)

$$X = P Z = P Q_D(t) \begin{pmatrix} c_1 \\ c_2 \\ \vdots \\ c_m \end{pmatrix} \quad - (9)$$

p242

(09.11.11)

$$X' = AX \quad A = \begin{pmatrix} 3 & 3 \\ 1 & 5 \end{pmatrix}$$

• diagonalization

(1) eigenvalues

$$\begin{vmatrix} 3-\lambda & 3 \\ 1 & 5-\lambda \end{vmatrix} = 0$$

$$\lambda = 2, \quad \lambda = 6$$

(2) eigenvectors

(i) $\lambda = 2$

$$\begin{pmatrix} 3 & 3 \\ 1 & 5 \end{pmatrix} \begin{pmatrix} a \\ b \end{pmatrix} = 2 \begin{pmatrix} a \\ b \end{pmatrix}$$

$$\vec{z}_1 = \begin{pmatrix} -3 \\ 1 \end{pmatrix}$$

(ii) $\lambda = 6$

$$\begin{pmatrix} 3 & 3 \\ 1 & 5 \end{pmatrix} \begin{pmatrix} a \\ b \end{pmatrix} = 6 \begin{pmatrix} a \\ b \end{pmatrix}$$

$$\vec{z}_2 = \begin{pmatrix} 1 \\ 1 \end{pmatrix}$$

(3) diagonalization

$$P = \begin{pmatrix} -3 & 1 \\ 1 & 1 \end{pmatrix}$$

$$D = \begin{pmatrix} 2 & 0 \\ 0 & 6 \end{pmatrix}$$

$$P^{-1} = -\frac{1}{4} \begin{pmatrix} 1 & -1 \\ -1 & -3 \end{pmatrix}$$

$$\Rightarrow A = P D P^{-1}$$

$$\Rightarrow X' = P D P^{-1} X$$

$$\Rightarrow P^{-1} X' = D P^{-1} X$$

$$\Rightarrow (P^{-1} X)' = D (P^{-1} X) \quad - \textcircled{1}$$

Put

$$Z = P^{-1} X \quad - \textcircled{2}$$

$$\textcircled{2} \rightarrow \textcircled{1}$$

$$Z' = D Z$$

$$Z = \begin{pmatrix} e^{2t} & 0 \\ 0 & e^{6t} \end{pmatrix} \begin{pmatrix} c_1 \\ c_2 \end{pmatrix} \quad - \textcircled{2}$$

$$\textcircled{3} \rightarrow \textcircled{2}$$

$$X = P Z$$

$$= \begin{pmatrix} -3 & 1 \\ 1 & 1 \end{pmatrix} \begin{pmatrix} e^{2t} & 0 \\ 0 & e^{6t} \end{pmatrix} \begin{pmatrix} c_1 \\ c_2 \end{pmatrix}$$

$$= \begin{pmatrix} -3e^{2t} & e^{6t} \\ e^{2t} & e^{6t} \end{pmatrix} \begin{pmatrix} c_1 \\ c_2 \end{pmatrix} \quad \times$$

* non-homogeneous differential Eq.

169

$$X' = AX + G \quad - ①$$

$$X = \Omega(t)C + \Psi_p(t) \quad - ②$$

$\Omega(t)C$: general solution of $X' = AX$

$\Psi_p(t)$: particular solution of $X' = AX + G$

How to derive $\Psi_p(t)$?

Put

$$\Psi_p(t) = \Omega(t)U(t) \quad - ③$$

③ \rightarrow ①

$$\underline{\Omega'(t)U(t) + \Omega(t)U'(t) = A\Omega(t)U(t) + G}$$

$= A\Omega(t)$

$$A\Omega(t)\cancel{U(t)} + \Omega(t)U'(t) = A\Omega(t)\cancel{U(t)} + G$$

$$U'(t) = \Omega^{-1}(t)G$$

$$\underline{U(t) = \int \Omega^{-1}(t)G dt} \quad - ④$$

④ \rightarrow ③

$$\boxed{\Psi_p(t) = \Omega(t) \int \Omega^{-1}(t)G dt}$$

*

(5/11/6.12)

$$X' = AX + B \quad A = \begin{pmatrix} 1 & -10 \\ -1 & 4 \end{pmatrix} \quad B = \begin{pmatrix} e^t \\ \sin t \end{pmatrix}$$

(i) General solution of homogeneous Equation

① Eigenvalues

$$\begin{vmatrix} 1-\lambda & -10 \\ -1 & 4-\lambda \end{vmatrix} = 0$$

$$\lambda = -1, 6$$

② Eigenvectors

$$(i) \lambda_1 = -1$$

$$\begin{pmatrix} 1 & -10 \\ -1 & 4 \end{pmatrix} \begin{pmatrix} a \\ b \end{pmatrix} = - \begin{pmatrix} a \\ b \end{pmatrix}$$

$$x_1 = \begin{pmatrix} 5 \\ 1 \end{pmatrix}$$

$$(ii) \lambda_2 = 6$$

$$\begin{pmatrix} 1 & -10 \\ -1 & 4 \end{pmatrix} \begin{pmatrix} a \\ b \end{pmatrix} = 6 \begin{pmatrix} a \\ b \end{pmatrix}$$

$$x_2 = \begin{pmatrix} -2 \\ 1 \end{pmatrix}$$

$$X_h = Q(t) \begin{pmatrix} c_1 \\ c_2 \end{pmatrix} \quad - (1)$$

$$Q(t) = \begin{pmatrix} 5e^{-t} & -2e^{6t} \\ e^{-t} & e^{6t} \end{pmatrix} \quad - (2)$$

$$Q^{-1}(t) = \frac{1}{7} \begin{pmatrix} e^t & 2e^t \\ -e^{-6t} & 5e^{-t} \end{pmatrix} \quad - (3)$$

$$\Omega^{-1}(t) B$$

$$= \frac{1}{7} \begin{pmatrix} e^t & 2e^t \\ -e^{6t} & 5e^{6t} \end{pmatrix} \begin{pmatrix} e^t \\ \sin t \end{pmatrix}$$

$$= \frac{1}{7} \begin{pmatrix} e^{2t} + 2 \sin t e^t \\ -e^{6t} + 5 \sin t e^{6t} \end{pmatrix} \quad - \textcircled{8}$$

$$\int (e^{2t} + 2 \sin t e^t) dt = \frac{1}{2} e^{2t} + e^t (\sin t - \cos t) \quad - \textcircled{9}$$

$$\int (-e^{6t} + 5 \sin t e^{6t}) dt = \frac{1}{6} e^{6t} - \frac{5}{37} e^{6t} (6 \sin t + \cos t)$$

* Formula

$$\int \sin t e^{at} dt = \frac{e^{at} [-\cos t + a \sin t]}{1+a^2}$$

$$\Rightarrow \int \Omega^{-1}(t) B(t) dt = \begin{pmatrix} \frac{1}{14} e^{2t} + \frac{1}{7} e^t (\sin t - \cos t) \\ \frac{1}{36} e^{6t} - \frac{5}{259} e^{6t} (6 \sin t + \cos t) \end{pmatrix} \quad - \textcircled{10}$$

Thus,

$$\begin{aligned} \Phi_p(t) &= \Omega(t) \int \Omega^{-1}(t) B(t) dt \\ &= \begin{pmatrix} \frac{3}{10} e^t + \frac{25}{37} \sin t - \frac{25}{37} \cos t \\ \frac{1}{10} e^t + \frac{1}{37} \sin t - \frac{6}{37} \cos t \end{pmatrix} \quad - \textcircled{11} \end{aligned}$$

Thus

$$X(t) = \begin{pmatrix} 5 e^t & -2e^{6t} \\ e^{-t} & e^{6t} \end{pmatrix} \begin{pmatrix} C_1 \\ C_2 \end{pmatrix} + \begin{pmatrix} \frac{3}{10} e^t + \frac{25}{37} \sin t - \frac{25}{37} \cos t \\ \frac{1}{10} e^t + \frac{1}{37} \sin t - \frac{6}{37} \cos t \end{pmatrix} //$$

* Matrix diagonalization

$$X' = AX + G \quad - (1)$$

$$A = PDP^{-1}$$

} - (2)

$$D = \begin{pmatrix} \lambda_1 & 0 & 0 & \dots & 0 \\ 0 & \lambda_2 & 0 & \dots & 0 \\ \vdots & \vdots & \vdots & \dots & \vdots \\ 0 & 0 & 0 & \dots & \lambda_m \end{pmatrix}$$

(2) \rightarrow (1)

$$X' = PDP^{-1}X + G$$

$$P^{-1} \times \parallel \quad P^{-1}X' = DP^{-1}X + P^{-1}G \quad - (3)$$

Put

$$Z = P^{-1}X \quad - (4)$$

(4) \rightarrow (3)

$$Z' = DZ + P^{-1}G \quad - (5)$$

$$\text{Let } Z = \begin{pmatrix} z_1 \\ z_2 \\ \vdots \\ z_m \end{pmatrix} \quad P^{-1}G = \begin{pmatrix} f_1(t) \\ f_2(t) \\ \vdots \\ f_m(t) \end{pmatrix}$$

Then

$$z_1' = \lambda_1 z_1 + f_1(t)$$

$$z_2' = \lambda_2 z_2 + f_2(t)$$

\vdots

$$z_m' = \lambda_m z_m + f_m(t)$$

Linear Eqn

$$\frac{dy}{dx} + p(x)y = Q(x)$$

$$y = e^{-\int p dx} \left[\int Q e^{\int p dx} dx + C \right]$$

(Ex 21.6.13)

$$X' = \begin{pmatrix} 3 & 3 \\ 1 & 5 \end{pmatrix} X + \begin{pmatrix} 8 \\ 4e^{3t} \end{pmatrix} \quad - \textcircled{1}$$

$$P = \begin{pmatrix} -3 & 1 \\ 1 & 1 \end{pmatrix} \quad D = \begin{pmatrix} 2 & 0 \\ 0 & 6 \end{pmatrix} \quad P^{-1} = -\frac{1}{4} \begin{pmatrix} 1 & -1 \\ -1 & -3 \end{pmatrix} \quad \} - \textcircled{2}$$

$$A = P D P^{-1}$$

 $\textcircled{2} \rightarrow \textcircled{1}$

$$X' = P D P^{-1} X + \begin{pmatrix} 8 \\ 4e^{3t} \end{pmatrix}$$

$$(P^{-1}X)' = D(P^{-1}X) + P^{-1} \begin{pmatrix} 8 \\ 4e^{3t} \end{pmatrix}$$

put

$$Z = P^{-1}X \quad - \textcircled{3}$$

Then

$$Z' = D Z + \begin{pmatrix} -2 + e^{3t} \\ 2 + 3e^{3t} \end{pmatrix} \quad - \textcircled{4}$$

$$\text{put } Z = \begin{pmatrix} z_1 \\ z_2 \end{pmatrix} \quad - \textcircled{5}$$

 $\textcircled{4} \rightarrow \textcircled{5}$

$$\begin{pmatrix} z_1' \\ z_2' \end{pmatrix} = \begin{pmatrix} 2 & 0 \\ 0 & 6 \end{pmatrix} \begin{pmatrix} z_1 \\ z_2 \end{pmatrix} + \begin{pmatrix} -2 + e^{3t} \\ 2 + 3e^{3t} \end{pmatrix}$$

$$\Rightarrow \left. \begin{aligned} z_1' &= 2z_1 + (-2 + e^{3t}) \\ z_2' &= 6z_2 + (2 + 3e^{3t}) \end{aligned} \right\} - \textcircled{6}$$

Solution

$$\begin{aligned} z_1(t) &= C_1 e^{2t} + e^{2t} + 1 \\ z_2(t) &= C_2 e^{6t} - e^{2t} - \frac{1}{2} \end{aligned} \quad - (1)$$

$$\Rightarrow Z(t) = \begin{pmatrix} C_1 e^{2t} + e^{2t} + 1 \\ C_2 e^{6t} - e^{2t} - \frac{1}{2} \end{pmatrix} \quad - (2)$$

 $(1) \rightarrow (2)$

$$X = P Z$$

$$= \begin{pmatrix} -3 & 1 \\ 1 & 1 \end{pmatrix} \begin{pmatrix} C_1 e^{2t} + e^{2t} + 1 \\ C_2 e^{6t} - e^{2t} - \frac{1}{2} \end{pmatrix}$$

$$= \begin{pmatrix} -3C_1 e^{2t} + C_2 e^{6t} - 4e^{2t} - \frac{10}{3} \\ C_1 e^{2t} + C_2 e^{6t} + \frac{2}{3} \end{pmatrix}$$

$$= \Omega(t) \begin{pmatrix} C_1 \\ C_2 \end{pmatrix} + \begin{pmatrix} -4e^{2t} - \frac{10}{3} \\ \frac{2}{3} \end{pmatrix} \quad - (3)$$

where

$$\Omega(t) = \begin{pmatrix} -3e^{2t} & e^{6t} \\ e^{2t} & e^{6t} \end{pmatrix} \quad - (4)$$

X

(5) 11.6.14)

$$X(0) = \begin{pmatrix} -3 & 1 \\ 1 & 1 \end{pmatrix} \begin{pmatrix} C_1 \\ C_2 \end{pmatrix} + \begin{pmatrix} -\frac{17}{2} \\ \frac{11}{2} \end{pmatrix} = \begin{pmatrix} 2 \\ -7 \end{pmatrix}$$

$$C_1 = -\frac{17}{4}, \quad C_2 = -\frac{41}{12}$$

$$X(t) = \begin{pmatrix} -3e^{2t} & e^{6t} \\ e^{2t} & e^{6t} \end{pmatrix} \begin{pmatrix} -\frac{17}{4} \\ -\frac{41}{12} \end{pmatrix} + \begin{pmatrix} -4e^{3t} - \frac{10}{2} \\ \frac{11}{2} \end{pmatrix} \quad \times$$